Move around things

erasure/theories/EEtaExpanded.v
@@ -7,6 +7,181 @@ From MetaCoq.PCUIC Require Import PCUICAst PCUICAstUtils
      PCUICConfluence PCUICConversion 
      PCUICCumulativity PCUICSR PCUICSafeLemmata
      PCUICValidity PCUICPrincipality PCUICElimination PCUICSN.
+     
+
+From MetaCoq.Template Require Import config utils BasicAst Universes.
+From MetaCoq.Erasure Require Import EAst ETyping EAstUtils.
+
+
+From MetaCoq.Erasure Require Import EWcbvEval.
+
+Lemma eval_trans' {wfl : WcbvFlags} {Σ e e' e''} :
+  eval Σ e e' -> eval Σ e' e'' -> e' = e''.
+Proof.
+  intros ev ev'.
+  eapply eval_to_value in ev.
+  eapply value_final in ev.
+  eapply (eval_deterministic ev ev').
+Qed.
+
+Lemma eval_trans {wfl : WcbvFlags} {Σ e e' e''} :
+  eval Σ e e' -> eval Σ e' e'' -> eval Σ e e''.
+Proof.
+  intros ev ev'.
+  enough (e' = e'') by now subst.
+  eapply eval_trans'; eauto.
+Qed.
+
+Arguments eval : clear implicits.
+
+Lemma eval_app_cong_tApp Σ t v args res :
+  eval target_wcbv_flags Σ t v ->  
+  eval target_wcbv_flags Σ (tApp v args) res ->
+  eval target_wcbv_flags Σ (tApp t args) res.
+Proof.
+  intros. depind H0.
+  - econstructor; eauto. eapply eval_trans; eauto.
+  - econstructor; eauto. eapply eval_trans; eauto.
+  - eapply eval_fix'; eauto. eapply eval_trans; eauto.
+  - eapply eval_app_cong; eauto. eapply eval_trans; eauto.
+  - cbn in i. easy.
+Qed.
+
+Definition isRel t :=
+    match t with tRel _ => true | _ => false end.
+
+Section expanded.
+
+Variable Σ : global_declarations.
+
+Local Unset Elimination Schemes.
+ 
+Inductive expanded (Γ : list nat): term -> Prop :=
+| expanded_tRel (n : nat) : nth n Γ 0 = 0 -> expanded Γ (tRel n)
+| expanded_tRel_app (n : nat) args : nth n Γ 0 <= #|args| -> Forall (expanded Γ) args -> expanded Γ (mkApps (tRel n) args)
+| expanded_tLambda (na : name) (body : term) : (* expanded Γ ty -> *) expanded (0 :: Γ) body -> expanded Γ (tLambda na body)
+| expanded_tLetIn (na : name) (def : term) (body : term) : expanded Γ def (* -> expanded Γ def_ty *) -> expanded (0 :: Γ) body -> expanded Γ (tLetIn na def body)
+| expanded_mkApps (f : term) (args : list term) : negb (isConstruct f || isFix f || isRel f) -> expanded Γ f -> Forall (expanded Γ) args -> expanded Γ (mkApps f args)
+| expanded_tConst (c : kername) : expanded Γ (tConst c)
+| expanded_tCase (ind : inductive) (pars : nat) (discr : term) (branches : list (list name × term)) :  
+    expanded Γ discr -> 
+    Forall (fun br => expanded (repeat 0 #|br.1| ++ Γ) br.2) branches -> 
+    expanded Γ (tCase (ind, pars) discr branches)
+| expanded_tProj (proj : projection) (t : term) : expanded Γ t -> expanded Γ (tProj proj t)
+| expanded_tFix (mfix : mfixpoint term) (idx : nat) args d : 
+  Forall (fun d => 
+           let ctx := rev_map (fun  d => 1 + d.(rarg)) mfix in
+          expanded (ctx ++ Γ) d.(dbody)) mfix ->
+  Forall (expanded Γ) args ->
+  args <> [] ->
+  nth_error mfix idx = Some d ->
+  #|args| > d.(rarg) ->
+  expanded Γ (mkApps (tFix mfix idx) args)
+| expanded_tCoFix (mfix : mfixpoint term) (idx : nat) : 
+  Forall (fun d => expanded (repeat 0 #|mfix| ++ Γ) d.(dbody)) mfix ->
+  expanded Γ (tCoFix mfix idx)
+| expanded_tConstruct_app ind idx mind idecl cname c args :
+    declared_constructor Σ (ind, idx) mind idecl (cname, c) ->
+    #|args| >= ind_npars mind + c -> 
+    Forall (expanded Γ) args ->
+    expanded Γ (mkApps (tConstruct ind idx) args)
+| expanded_tBox : expanded Γ tBox.
+
+End expanded.
+
+Lemma expanded_ind :
+  ∀ (Σ : global_declarations) (P : list nat → term → Prop),
+    (∀ (Γ : list nat) (n : nat), nth n Γ 0 = 0 → P Γ (tRel n))
+    → (∀ (Γ : list nat) (n : nat) (args : list term),
+	        nth n Γ 0 ≤ #|args|
+        → Forall (expanded Σ Γ) args
+        → Forall (P Γ) args 
+        → P Γ (mkApps (tRel n) args))
+    → (∀ (Γ : list nat) (na : name) (body : term),
+          expanded Σ (0 :: Γ) body → P (0 :: Γ) body → P Γ (tLambda na body))
+    → (∀ (Γ : list nat) (na : name) (def body : term),
+          expanded Σ Γ def
+        → P Γ def
+        → expanded Σ (0 :: Γ) body
+        → P (0 :: Γ) body → P Γ (tLetIn na def body))
+    → (∀ (Γ : list nat) (f3 : term) (args : list term),
+          negb (isConstruct f3 || isFix f3 || isRel f3)
+        → expanded Σ Γ f3
+        → P Γ f3 → Forall (expanded Σ Γ) args → Forall (P Γ) args → P Γ (mkApps f3 args))
+    → (∀ (Γ : list nat) (c : kername), P Γ (tConst c))
+    → (∀ (Γ : list nat) (ind : inductive) 
+         (pars : nat) (discr : term) (branches : 
+                                     list 
+                                       (list name × term)),
+          expanded Σ Γ discr
+        → P Γ discr
+        → Forall
+            (λ br : list name × term,
+                expanded Σ (repeat 0 #|br.1| ++ Γ) br.2) branches
+        → Forall
+            (λ br : list name × term,
+                P (repeat 0 #|br.1| ++ Γ) br.2) branches
+        → P Γ (tCase (ind, pars) discr branches))
+    → (∀ (Γ : list nat) (proj : projection) (t : term),
+          expanded Σ Γ t → P Γ t → P Γ (tProj proj t))
+    → (∀ (Γ : list nat) (mfix : mfixpoint term) 
+         (idx : nat) (args : list term) 
+         (d : def term),
+          Forall
+            (λ d0 : def term,
+                let ctx := rev_map (fun  d => 1 + d.(rarg)) mfix in
+                expanded Σ (ctx ++ Γ) (dbody d0)) mfix
+          → Forall
+            (λ d0 : def term,
+               let ctx := rev_map (fun  d => 1 + d.(rarg)) mfix in
+                P (ctx ++ Γ) (dbody d0)) mfix
+          → Forall (expanded Σ Γ) args
+          → Forall (P Γ) args
+          → args ≠ []
+          → nth_error mfix idx = Some d
+          → #|args| > rarg d
+                    → P Γ (mkApps (tFix mfix idx) args))
+    → (∀ (Γ : list nat) (mfix : mfixpoint term) (idx : nat),
+          Forall
+            (λ d : def term,
+                expanded Σ (repeat 0 #|mfix| ++ Γ) (dbody d)) mfix 
+        → Forall
+            (λ d : def term,
+                P (repeat 0 #|mfix| ++ Γ) (dbody d)) mfix 
+        → P Γ (tCoFix mfix idx))
+    → (∀ (Γ : list nat) (ind : inductive) 
+         (idx : nat) (mind : mutual_inductive_body) 
+         (idecl : one_inductive_body) 
+         (cname : ident) (c : nat) 
+         (args : list term),
+          declared_constructor Σ (ind, idx) mind idecl (cname, c)
+        → #|args| ≥ ind_npars mind + c
+        → Forall (expanded Σ Γ) args
+        → Forall (P Γ) args
+        → P Γ (mkApps (tConstruct ind idx) args))
+    → (∀ Γ : list nat, P Γ tBox)
+    → ∀ (Γ : list nat) (t : term), expanded Σ Γ t → P Γ t.
+Proof.
+  intros Σ P HRel HRel_app HLamdba HLetIn HmkApps HConst HCase HProj HFix HCoFix HConstruct HBox.
+  fix f 3.
+  intros Γ t Hexp.  destruct Hexp; eauto.
+  - eapply HRel_app; eauto. clear - f H0. induction H0; econstructor; eauto.
+  - eapply HmkApps; eauto. clear - f H0. induction H0; econstructor; eauto.
+  - eapply HCase; eauto. induction H; econstructor; eauto.
+  - assert (Forall (P Γ) args). { clear - H0 f. induction H0; econstructor; eauto. }
+    eapply HFix; eauto.
+    revert H. clear - f.
+    generalize mfix at 1 3. intros mfix0 H.  induction H; econstructor; cbn in *; eauto; split.
+  - eapply HCoFix; eauto.
+    revert H. clear - f.
+    generalize mfix at 1 3. intros mfix0 H.  induction H; econstructor; cbn in *; eauto; split.
+  - eapply HConstruct; eauto.
+    clear - H1 f. induction H1; econstructor; eauto.
+Qed.
+
+
+
+Local Hint Constructors expanded : core.
 
 From MetaCoq.SafeChecker Require Import PCUICWfEnv.
      
@@ -80,20 +255,23 @@ Proof.
   intros [->|hin]. lia. specialize (IHl hin); lia.
 Qed.
 
-Equations discr_construct_fix (t : term) : Prop :=
-  discr_construct_fix (tConstruct ind n) := False ;
-  discr_construct_fix (tFix mfix idx) := False ;
-  discr_construct_fix _ := True.
+Equations discr_expanded_head (t : term) : Prop :=
+  discr_expanded_head (tConstruct ind n) := False ;
+  discr_expanded_head (tFix mfix idx) := False ;
+  discr_expanded_head (tRel n) := False ;
+  discr_expanded_head _ := True.
 
-Inductive construct_fix_view : term -> Type :=
-| ccview_construct : forall ind n, construct_fix_view (tConstruct ind n)
-| ccview_fix : forall mfix idx, construct_fix_view (tFix mfix idx)
-| ccview_other : forall t, discr_construct_fix t -> construct_fix_view t.
+Inductive expanded_head_view : term -> Type :=
+| expanded_head_construct : forall ind n, expanded_head_view (tConstruct ind n)
+| expanded_head_fix : forall mfix idx, expanded_head_view (tFix mfix idx)
+| expanded_head_rel : forall n, expanded_head_view (tRel n)
+| expanded_head_other : forall t, discr_expanded_head t -> expanded_head_view t.
 
-Equations cc_viewc t : construct_fix_view t :=
-  cc_viewc (tConstruct ind n) := ccview_construct ind n ;
-  cc_viewc (tFix mfix idx) := ccview_fix mfix idx ;
-  cc_viewc t := ccview_other t I.
+Equations expanded_head_viewc t : expanded_head_view t :=
+  expanded_head_viewc (tConstruct ind n) := expanded_head_construct ind n ;
+  expanded_head_viewc (tFix mfix idx) := expanded_head_fix mfix idx ;
+  expanded_head_viewc (tRel n) := expanded_head_rel n ;
+  expanded_head_viewc t := expanded_head_other t I.
 
 Lemma In_All {A} {P : A -> Type} l : 
     (∀ x : A, In x l -> P x) -> All P l.
@@ -145,21 +323,23 @@ Section isEtaExp.
     
   Import TermSpineView.
 
-  Equations? isEtaExp (e : EAst.term) : bool
+  Equations? isEtaExp (Γ : list nat) (e : EAst.term) : bool
     by wf e (fun x y : EAst.term => size x < size y) :=
-  | e with TermSpineView.view e := {
-    | tRel i => true
-    | tEvar ev args => forallb_InP args (fun x H => isEtaExp x)
-    | tLambda na M => isEtaExp M
-    | tApp u v napp nnil with cc_viewc u := 
-      { | ccview_construct ind i => isEtaExp_app ind i (List.length v) && forallb_InP v (fun x H => isEtaExp x)
-        | ccview_fix mfix idx => isEtaExp_fixapp mfix idx (List.length v) && forallb_InP mfix (fun x H => isEtaExp x.(dbody)) && forallb_InP v (fun x H => isEtaExp x)
-        | ccview_other _ _ => isEtaExp u && forallb_InP v (fun x H => isEtaExp x) }
-    | tLetIn na b b' => isEtaExp b && isEtaExp b'
-    | tCase ind c brs => isEtaExp c && forallb_InP brs (fun x H => isEtaExp x.2)
-    | tProj p c => isEtaExp c
-    | tFix mfix idx => (* forallb_InP mfix (fun x H => isEtaExp x.(dbody)) *) false
-    | tCoFix mfix idx => forallb_InP mfix (fun x H => isEtaExp x.(dbody))
+    isEtaExp Γ e with TermSpineView.view e := {
+    | tRel i => Nat.eqb (nth i Γ 0) 0
+    | tEvar ev args => forallb_InP args (fun x H => isEtaExp Γ x)
+    | tLambda na M => isEtaExp (0 :: Γ) M
+    | tApp u v napp nnil with expanded_head_viewc u := 
+      { | expanded_head_construct ind i => isEtaExp_app ind i (List.length v) && forallb_InP v (fun x H => isEtaExp Γ x)
+        | expanded_head_fix mfix idx => isEtaExp_fixapp mfix idx (List.length v) && 
+                                        forallb_InP mfix (fun x H => isEtaExp (rev_map (S ∘ rarg) mfix ++ Γ) x.(dbody)) && forallb_InP v (fun x H => isEtaExp Γ x)
+        | expanded_head_rel n => (nth n Γ 0 <=? List.length v) && forallb_InP v (fun x H => isEtaExp Γ x) 
+        | expanded_head_other _ _ => isEtaExp Γ u && forallb_InP v (fun x H => isEtaExp Γ x) }
+    | tLetIn na b b' => isEtaExp Γ b && isEtaExp (0 :: Γ) b'
+    | tCase ind c brs => isEtaExp Γ c && forallb_InP brs (fun x H => isEtaExp (repeat 0 #|x.1| ++ Γ) x.2)
+    | tProj p c => isEtaExp Γ c
+    | tFix mfix idx => false
+    | tCoFix mfix idx => forallb_InP mfix (fun x H => isEtaExp (repeat 0 #|mfix| ++ Γ) x.(dbody))
     | tBox => true
     | tVar _ => true
     | tConst _ => true
@@ -173,6 +353,9 @@ Section isEtaExp.
       now apply (In_size id size).
     - rewrite size_mkApps.
       apply (In_size id (fun d => size d.(dbody))) in H. unfold id in H. 
+      change (fun x => size x) with size in H. cbn. lia.
+    - rewrite size_mkApps.
+      apply (In_size id size) in H. unfold id in H. 
       change (fun x => size x) with size in H. cbn. lia.
     - rewrite size_mkApps.
       apply (In_size id size) in H. unfold id in H. 
@@ -195,18 +378,19 @@ Section isEtaExp.
 
   Hint Rewrite @forallb_InP_spec : isEtaExp.
 
-  Lemma isEtaExp_mkApps_nonnil f v :
+  Lemma isEtaExp_mkApps_nonnil Γ f v :
     ~~ isApp f -> v <> [] ->
-    isEtaExp (mkApps f v) = match cc_viewc f with 
-      | ccview_construct ind i => isEtaExp_app ind i #|v| && forallb isEtaExp v
-      | ccview_fix mfix idx => isEtaExp_fixapp mfix idx #|v| && forallb_InP mfix (fun x H => isEtaExp x.(dbody)) && forallb isEtaExp v
-      | ccview_other t discr => isEtaExp f && forallb isEtaExp v
+    isEtaExp Γ (mkApps f v) = match expanded_head_viewc f with 
+      | expanded_head_construct ind i => isEtaExp_app ind i #|v| && forallb (isEtaExp Γ) v
+      | expanded_head_fix mfix idx => isEtaExp_fixapp mfix idx #|v| && forallb (fun x => isEtaExp (rev_map (S ∘ rarg) mfix ++ Γ) x.(dbody)) mfix && forallb (isEtaExp Γ) v
+      | expanded_head_rel n => (nth n Γ 0 <=? List.length v) && forallb (fun x => isEtaExp Γ x) v
+      | expanded_head_other t discr => isEtaExp Γ f && forallb (isEtaExp Γ) v
     end.
   Proof.
     rewrite isEtaExp_equation_1.
     intros napp hv.
     destruct (TermSpineView.view_mkApps (TermSpineView.view (mkApps f v)) napp hv) as [hna [hv' ->]].
-    cbn. destruct (cc_viewc f); cbn; simp isEtaExp => //.
+    cbn. destruct (expanded_head_viewc f); cbn; simp isEtaExp => //.
   Qed.
 
   Tactic Notation "simp_eta" "in" hyp(H) := simp isEtaExp in H; rewrite -?isEtaExp_equation_1 in H.
@@ -214,159 +398,383 @@ Section isEtaExp.
 
   Definition is_cons {A} (l : list A) := match l with [] => false | _ => true end.
   
-  Lemma isEtaExp_mkApps f v : ~~ isApp f -> 
-    isEtaExp (mkApps f v) = match cc_viewc f with 
-      | ccview_construct ind i => isEtaExp_app ind i #|v| && forallb isEtaExp v
-      | ccview_fix mfix idx => isEtaExp_fixapp mfix idx #|v| && forallb_InP mfix (fun x H => isEtaExp x.(dbody)) && forallb isEtaExp v
-      | ccview_other t discr => isEtaExp f && forallb isEtaExp v
+  Lemma isEtaExp_mkApps Γ f v : ~~ isApp f -> 
+    isEtaExp Γ (mkApps f v) = match expanded_head_viewc f with 
+      | expanded_head_construct ind i => isEtaExp_app ind i #|v| && forallb (isEtaExp Γ) v
+      | expanded_head_fix mfix idx => isEtaExp_fixapp mfix idx #|v| && forallb (fun x => isEtaExp (rev_map (S ∘ rarg) mfix ++ Γ) x.(dbody)) mfix && forallb (isEtaExp Γ) v
+      | expanded_head_rel n => (nth n Γ 0 <=? List.length v) && forallb (fun x => isEtaExp Γ x) v
+      | expanded_head_other t discr => isEtaExp Γ f && forallb (isEtaExp Γ) v
     end.
   Proof.
     intros napp.
     destruct v using rev_case; simp_eta.
-    - destruct cc_viewc; rewrite ? andb_true_r //. cbn. unfold isEtaExp_fixapp. now destruct (nth_error); cbn.
-    - rewrite isEtaExp_mkApps_nonnil //. destruct v; cbn; try congruence.
+    - destruct expanded_head_viewc; rewrite ? andb_true_r //. cbn. unfold isEtaExp_fixapp. now destruct (nth_error); cbn.
+      cbn. destruct (Nat.eqb_spec (nth n Γ 0) 0), (Nat.leb_spec (nth n Γ 0) 0); try reflexivity; lia.
+    - rewrite isEtaExp_mkApps_nonnil //. destruct v; cbn; try congruence.      
   Qed.
 
-  Lemma isEtaExp_Constructor ind i v :
-    isEtaExp (mkApps (EAst.tConstruct ind i) v) = isEtaExp_app ind i #|v| && forallb isEtaExp v.
+  Lemma isEtaExp_Constructor Γ ind i v :
+    isEtaExp Γ (mkApps (EAst.tConstruct ind i) v) = isEtaExp_app ind i #|v| && forallb (isEtaExp Γ) v.
   Proof.
     now rewrite isEtaExp_mkApps.
   Qed.
-
-  Lemma isEtaExp_mkApps_intro t l : isEtaExp t -> All isEtaExp l -> isEtaExp (mkApps t l).
+ 
+  Lemma isEtaExp_mkApps_intro Γ t l : isEtaExp Γ t -> All (isEtaExp Γ) l -> isEtaExp Γ (mkApps t l).
   Proof.
-    revert t; induction l using rev_ind; auto.
-    intros t et a; eapply All_app in a as [].
+    revert t Γ; induction l using rev_ind; auto.
+    intros t Γ et a; eapply All_app in a as [].
     depelim a0. clear a0.
     destruct (decompose_app t) eqn:da.
     rewrite (decompose_app_inv da) in et *.
     pose proof (decompose_app_notApp _ _ _ da).
     destruct l0. simp_eta.
     - rewrite isEtaExp_mkApps //.
-      destruct cc_viewc.
+      destruct expanded_head_viewc.
       + cbn. len.
         rtoProp; repeat solve_all. cbn in et. simp isEtaExp in et.
-        eapply isEtaExp_app_mon; tea; lia.
+        eapply isEtaExp_app_mon; tea; lia. 
         eapply All_app_inv; eauto.
       + cbn in *; congruence.
+      + simp_eta in et. eapply Nat.eqb_eq in et. rewrite et.
+        rtoProp. split. cbn. eauto.
+        solve_all. eapply All_app_inv; solve_all.
       + rewrite et forallb_app /=. rtoProp; repeat solve_all. 
     - rewrite isEtaExp_mkApps in et => //.
-      destruct cc_viewc.
+      destruct expanded_head_viewc.
       + rewrite -mkApps_app. rewrite isEtaExp_Constructor.
         cbn. cbn. rtoProp; solve_all.
         eapply isEtaExp_app_mon; tea. cbn. len. lia. now depelim H1.
         depelim H1. solve_all. eapply All_app_inv => //.
         eapply All_app_inv => //. eauto.
-      + rewrite -mkApps_app. rewrite isEtaExp_mkApps //. simp cc_viewc.
-        rewrite forallb_InP_spec /isEtaExp_fixapp in et |- *.
+      + rewrite -mkApps_app. rewrite isEtaExp_mkApps //. simp expanded_head_viewc.
+        rewrite /isEtaExp_fixapp in et |- *.
         rtoProp; repeat split.
         * destruct nth_error; try congruence. eapply Nat.ltb_lt. eapply Nat.ltb_lt in H0.
           cbn in H0. len. lia.
         * solve_all.
-        * solve_all. eapply All_app_inv; solve_all. eapply All_app_inv; solve_all. 
+        * solve_all. eapply All_app_inv; solve_all. eapply All_app_inv; solve_all.
       + rewrite -mkApps_app. rewrite isEtaExp_mkApps //.
-        destruct (cc_viewc t0) => //.
+        cbn [expanded_head_viewc]. rtoProp. split.
+        cbn. eapply Nat.leb_le in H0. eapply Nat.leb_le. revert H0. len. lia.
+        solve_all. eapply All_app_inv. 2: eapply All_app_inv. all: solve_all.
+      + rewrite -mkApps_app. rewrite isEtaExp_mkApps //.
+        destruct (expanded_head_viewc t0) => //.
         move/andP: et => [] -> /=. rtoProp; solve_all.
         rewrite forallb_app. rtoProp; repeat solve_all.
         eapply All_app_inv; eauto.
   Qed.
 
-  Lemma etaExp_csubst a k b : 
-    isEtaExp a -> isEtaExp b -> isEtaExp (ECSubst.csubst a k b).
+  Hint Rewrite repeat_length : len.
+
+  Lemma expanded_lift Γ' Γ'' Γ t :
+    isEtaExp (Γ' ++ Γ)%list t ->
+    isEtaExp (Γ' ++ Γ'' ++ Γ)%list (lift #|Γ''| #|Γ'| t).
   Proof.
-    funelim (isEtaExp b); try simp_eta; eauto;
-      try toAll; repeat solve_all.
-    - intros. simp isEtaExp ; cbn. destruct Nat.compare => //. simp_eta in H.
-    - move/andP: H2 => [] etab etab'.
+  Admitted.
+
+  Lemma etaExp_csubst' a k b n Γ Δ : 
+    #|Γ| = k ->
+    closed a -> isEtaExp [] a -> isEtaExp (Γ ++ [n] ++ Δ) b -> isEtaExp (Γ ++ Δ) (ECSubst.csubst a k b).
+  Proof.
+    intros Hk Hcl. 
+    remember (Γ ++ [n] ++ Δ)%list as Γ_.
+    funelim (isEtaExp Γ_ b); try simp_eta; eauto; try fold csubst;
+      try toAll; repeat solve_all; subst.
+    - intros. simp isEtaExp ; cbn. destruct (Nat.compare_spec #|Γ0| i) => //; simp_eta.
+      + setoid_rewrite <- lift_closed.
+        rewrite <- (app_nil_r (Γ0 ++ Δ)).
+        eapply expanded_lift with(Γ' := []); eassumption. 
+        eassumption.
+      + rewrite app_nth2. lia.
+        rewrite app_nth2 in H0. lia.
+        eapply Nat.eqb_eq in H0. eapply Nat.eqb_eq.
+        rewrite <- H0 at 2. destruct i. lia.
+        cbn [Nat.pred].
+        rewrite app_nth2. cbn. lia. f_equal. cbn. lia.
+      + rewrite !app_nth1 in H0 |- *; try lia.
+        eapply Nat.eqb_eq in H0. eapply Nat.eqb_eq. lia.
+    - eapply H with (Γ := 0 :: Γ0); cbn; eauto.
+    - move/andP: H2 => [] etab etab'. simp_eta.
       apply/andP. split; eauto.
+      eapply H0 with (Γ := 0 :: Γ0); cbn; eauto.
     - rtoProp. intuition eauto.
-      solve_all.
-    - move/andP: H1 => [] etaexp h.
+      solve_all. rewrite app_assoc. eapply a0; cbn; eauto. now len. cbn.
+      now rewrite app_assoc.
+    - rewrite app_assoc. eapply a0; len; eauto. now rewrite app_assoc.
+    - fold csubst. move/andP: H1 => [] etaexp h.
       rewrite csubst_mkApps /=.
       rewrite isEtaExp_Constructor. solve_all.
       rewrite map_length. rtoProp; solve_all. solve_all.
     - rewrite csubst_mkApps /=.
       move/andP : H2 => [] /andP [] eu ef ev.
       rewrite isEtaExp_mkApps //.
-      simp cc_viewc.
+      simp expanded_head_viewc.
       rtoProp; repeat split.
       + rewrite /isEtaExp_fixapp in eu |- *. rewrite nth_error_map. destruct nth_error; try congruence.
         cbn. now len.
-      + rewrite forallb_InP_spec. solve_all.
       + solve_all.
+        rewrite app_assoc.  eapply a0; len; eauto. cbn. f_equal.
+        rewrite app_assoc. do 2 f_equal.
+        rewrite !rev_map_spec. f_equal. rewrite map_map. now eapply map_ext.      
+      + solve_all.
+    - rewrite csubst_mkApps /=. rtoProp. destruct (Nat.compare_spec #|Γ0| n) => //; simp_eta.
+      + eapply isEtaExp_mkApps_intro => //. 2: solve_all.
+        setoid_rewrite <- lift_closed.
+        rewrite <- (app_nil_r (Γ0 ++ Δ)).
+        eapply expanded_lift with(Γ' := []); eassumption. 
+        eassumption.
+      + rewrite isEtaExp_mkApps; eauto. cbn [expanded_head_viewc].
+        rtoProp. split. 2: solve_all.
+        eapply Nat.leb_le in H1. eapply Nat.leb_le. rewrite app_nth2 in H1 |- *; try lia.
+        len. rewrite <- H1. rewrite !app_nth2; cbn; try lia.
+        eapply Nat.eq_le_incl. f_equal. lia.
+      + rewrite isEtaExp_mkApps; eauto. cbn [expanded_head_viewc].
+        rtoProp. split. 2: solve_all. rewrite app_nth1 in H1 |- *; try lia.
+        eapply Nat.leb_le in H1. eapply Nat.leb_le. 
+        len. rewrite <- H1. rewrite !app_nth1; cbn; try lia.
     - rewrite csubst_mkApps /=.
       move/andP: H2 => [] eu ev.
-      specialize (H _ k H1 eu).
-      eapply isEtaExp_mkApps_intro => //. solve_all.
+      eapply isEtaExp_mkApps_intro => //. 2: solve_all.
+      eauto. 
+  Qed.
+
+  Lemma etaExp_csubst a b n : 
+    closed a -> isEtaExp []a -> isEtaExp [n] b -> isEtaExp [] (ECSubst.csubst a 0 b).
+  Proof.
+    intros.
+    eapply etaExp_csubst' with (Γ := []); eauto.
+  Qed.
+
+  Lemma etaExp_fixsubst k b Γ Δ mfix idx d : 
+    #|Γ| = k ->
+    nth_error mfix idx = Some d ->
+    closed (EAst.tFix mfix idx) ->
+    forallb (fun x => isEtaExp (rev_map (S ∘ rarg) mfix) x.(dbody)) mfix ->
+    isEtaExp (Γ ++ [1 + d.(EAst.rarg)] ++ Δ) b -> isEtaExp (Γ ++ Δ) (ECSubst.csubst (EAst.tFix mfix idx) k b).
+  Proof.
+    intros Hk Hnth Hcl. 
+    remember (Γ ++ [1 + d.(EAst.rarg)] ++ Δ)%list as Γ_.
+    funelim (isEtaExp Γ_ b); try simp_eta; eauto; try fold csubst;
+      try toAll; try now repeat solve_all; subst.
+    - intros. simp isEtaExp ; cbn. destruct (Nat.compare_spec #|Γ0| i) => //; simp_eta.
+      + rewrite app_nth2 in H0; try lia. subst. rewrite minus_diag in H0. now cbn in H0.
+      + rewrite app_nth2. lia.
+        rewrite app_nth2 in H0. lia.
+        eapply Nat.eqb_eq in H0. eapply Nat.eqb_eq.
+        rewrite <- H0 at 2. destruct i. lia.
+        cbn [Nat.pred].
+        rewrite app_nth2. cbn. lia. f_equal. cbn. lia.
+      + rewrite !app_nth1 in H0 |- *; try lia.
+        eapply Nat.eqb_eq in H0. eapply Nat.eqb_eq. lia.
+    - intros. solve_all. eapply a; eauto. solve_all.
+    - eapply H with (Γ := 0 :: Γ0); cbn -[isEtaExp]; eauto. 
+    - solve_all. move/andP: H2 => [] etab etab'. simp_eta.
+      apply/andP. split; eauto.
+      eapply H0 with (Γ := 0 :: Γ0); cbn; eauto.
+    - solve_all. rtoProp. intuition eauto.
+      solve_all. rewrite app_assoc. eapply a; cbn-[isEtaExp]; eauto. now len. cbn.
+      now rewrite app_assoc.
+      solve_all.
+    - solve_all. rewrite app_assoc. solve_all.  eapply a; len; eauto.
+      { cbn in Hcl. solve_all. rewrite Nat.add_0_r in a0. eauto. }
+      now rewrite app_assoc.
+      solve_all.
+    - solve_all. fold csubst. move/andP: H1 => [] etaexp h.
+      rewrite csubst_mkApps /=.
+      rewrite isEtaExp_Constructor. solve_all.
+      rewrite map_length. rtoProp; solve_all.
+      solve_all.
+      eapply a; eauto.
+      solve_all.
+    - solve_all. rewrite csubst_mkApps /=.
+      move/andP : H2 => [] /andP [] eu ef ev.
+      rewrite isEtaExp_mkApps //.
+      simp expanded_head_viewc.
+      rtoProp; repeat split.
+      + rewrite /isEtaExp_fixapp in eu |- *. rewrite nth_error_map.
+        destruct (nth_error mfix idx); try congruence.
+        cbn. now len.
+      + solve_all.
+        rewrite app_assoc.  eapply a; len; eauto.
+        { cbn in Hcl. solve_all. rewrite Nat.add_0_r in a0. eauto. }
+        cbn. f_equal.
+        rewrite app_assoc. do 2 f_equal.
+        rewrite !rev_map_spec. f_equal. rewrite map_map. now eapply map_ext.
+        solve_all.      
+      + solve_all. eapply a; eauto. solve_all.
+    - rewrite csubst_mkApps /=. rtoProp. destruct (Nat.compare_spec #|Γ0| n) => //; simp_eta.
+      + rewrite isEtaExp_mkApps => //. cbn [expanded_head_viewc].
+        rtoProp. repeat split; eauto.
+        * unfold isEtaExp_fixapp. rewrite Hnth. len. destruct H2 as [Hn H2].
+          subst. rewrite app_nth2 in Hn; try lia.
+          rewrite minus_diag in Hn. cbn in Hn. eapply Nat.ltb_lt.
+          eapply Nat.leb_le in Hn. lia.        
+        * cbn in Hcl. solve_all. 
+          setoid_rewrite <- lift_closed.
+          rewrite <- (app_nil_r (Γ0 ++ Δ)). 
+          eapply expanded_lift. now rewrite app_nil_r.
+          eapply closed_upwards. eassumption. now len.
+        * destruct H2. solve_all. eapply a ;eauto. solve_all.          
+      + rewrite isEtaExp_mkApps; eauto. cbn [expanded_head_viewc].
+        rtoProp. intros. destruct H2. split. 2:{ solve_all. eapply a; eauto. solve_all. }
+        eapply Nat.leb_le in H2. eapply Nat.leb_le. rewrite app_nth2 in H2 |- *; try lia.
+        len. rewrite <- H2. rewrite !app_nth2; cbn; try lia.
+        eapply Nat.eq_le_incl. destruct (n - #|Γ0|) eqn:E. lia. f_equal. lia.
+      + rewrite isEtaExp_mkApps; eauto. cbn [expanded_head_viewc].
+        intros. destruct H2.
+        rtoProp. split. 2:{ solve_all. eapply a; eauto. solve_all. }
+        rewrite app_nth1 in H2 |- *; try lia.
+        eapply Nat.leb_le in H2. eapply Nat.leb_le. 
+        len. rewrite <- H2. rewrite !app_nth1; cbn; try lia.
+    - intros. rtoProp. rewrite csubst_mkApps /=.
+      eapply isEtaExp_mkApps_intro => //. 2:{ solve_all. eapply a; eauto. solve_all. }
+      eapply H; eauto.
   Qed.
   
-  Lemma isEtaExp_substl s t : 
-    forallb isEtaExp s -> isEtaExp t ->
-    isEtaExp (substl s t).
+  Lemma isEtaExp_substl Γ Δ s t : 
+    #|Γ| = #|s| ->
+    Forall (closedn 0) s ->
+    forallb (isEtaExp []) s -> isEtaExp (Γ ++ Δ) t ->
+    isEtaExp Δ (substl s t).
   Proof.
-    induction s in t |- *; simpl; auto. rtoProp; intuition eauto using etaExp_csubst.
+    induction s in Γ, t |- *; simpl; auto;
+    rtoProp; intuition eauto using etaExp_csubst.
+    - destruct Γ; eauto; cbn in *; lia.
+    - invs H0. destruct Γ; cbn in H; invs H.
+      eapply IHs; eauto. eapply etaExp_csubst' with (Γ := []); eauto.
+  Qed.
+
+  Lemma isEtaExp_fixsubstl Δ mfix idx t : 
+    closed (EAst.tFix mfix idx) ->
+    forallb (fun x => isEtaExp (rev_map (S ∘ rarg) mfix) x.(dbody)) mfix ->
+    isEtaExp ((rev_map (S ∘ rarg) mfix) ++ Δ) t ->
+    isEtaExp Δ (substl (fix_subst mfix) t).
+  Proof.
+    intros Hcl Hall Heta.
+    cbn in Hcl. solve_all.
+    unfold fix_subst.
+    revert Hall Heta.
+  
+    generalize (@eq_refl _ mfix).
+    setoid_rewrite <- app_nil_r at 1.
+    generalize ((@nil (EAst.def EAst.term))).
+    generalize (mfix) at 1 6 8.
+    
+    intros mfix0. revert mfix Δ t.
+    induction mfix0  using rev_ind; intros.
+    - cbn -[isEtaExp] in *. eauto.
+    - cbn -[isEtaExp] in *. rewrite app_length Nat.add_comm. cbn -[substl isEtaExp].
+      eapply IHmfix0. 
+      + subst. now rewrite <- app_assoc.
+      + solve_all.
+      + eapply etaExp_fixsubst with (Γ := []); eauto.
+        2: cbn; solve_all. 2: solve_all.
+        2:{ cbn -[isEtaExp] in *. revert Heta.
+            rewrite !rev_map_spec map_app rev_app_distr. cbn -[isEtaExp] in *. intros.
+            exact Heta.
+        }
+        subst. rewrite <- app_assoc. cbn. now eapply nth_error_snoc.
   Qed.
 
   Lemma isEtaExp_iota_red pars args br :
-    forallb isEtaExp args ->
-    isEtaExp br.2 ->
-    isEtaExp (ETyping.iota_red pars args br).
+    Forall (closedn 0) args ->
+    forallb (isEtaExp []) args ->
+    isEtaExp (repeat 0 (#|args| - pars)) br.2 ->
+    isEtaExp [] (ETyping.iota_red pars args br).
   Proof.
-    intros etaargs etabr.
+    intros  Hcl etaargs etabr.
     unfold ETyping.iota_red.
-    rewrite isEtaExp_substl // forallb_rev forallb_skipn //.
+    erewrite (isEtaExp_substl _ []); eauto.
+    - shelve.
+    - solve_all. eapply All_skipn. solve_all.
+    - rewrite forallb_rev forallb_skipn //.
+    - rewrite app_nil_r. eauto.
+    Unshelve. len. now rewrite List.skipn_length.  
   Qed.
-  (* 
+   
+(*
+
   Lemma isEtaExp_fix_subst mfix : 
-    forallb (isEtaExp ∘ dbody) mfix ->
-    forallb isEtaExp (ETyping.fix_subst mfix).
+    forallb (isEtaExp (repeat 0 #|mfix|) ∘ dbody) mfix ->
+    forallb (isEtaExp []) (ETyping.fix_subst mfix).
   Proof.
     unfold ETyping.fix_subst.
     generalize (@eq_refl _ #|mfix|). 
-    generalize #|mfix| at 1 3.
-    solve_all. solve_all. revert n H.
+    generalize #|mfix| at 1 3 4.
+    intros. solve_all. revert n H H0.
     induction n; intros; simp_eta; constructor; auto.
+    + simp_eta.
     simp isEtaExp. solve_all. 
   Qed. 
- *)
+
+  *)
+ 
   Lemma isEtaExp_cofix_subst mfix : 
-    forallb (isEtaExp ∘ dbody) mfix ->
-    forallb isEtaExp (ETyping.cofix_subst mfix).
+    forallb (isEtaExp (repeat 0 #|mfix|) ∘ dbody) mfix ->
+    forallb (isEtaExp []) (ETyping.cofix_subst mfix).
   Proof.
-    unfold ETyping.cofix_subst. generalize #|mfix|.
-    solve_all. solve_all. revert n.
-    induction n; intros; simp_eta; constructor; auto.
-    simp isEtaExp. solve_all.
-  Qed.
+    intros. solve_all.
+    unfold ETyping.cofix_subst.
+    unfold cofix_subst. generalize #|mfix|. intros n. solve_all. induction n.
+      + econstructor.
+      + econstructor. simp_eta. solve_all. now rewrite app_nil_r. solve_all.
+  Qed. 
   
   Lemma isEtaExp_cunfold_fix mfix idx n f : 
-    forallb (isEtaExp ∘ dbody) mfix ->
+    forallb (closedn 0 ∘ dbody) mfix ->
+    forallb (isEtaExp (rev_map (S ∘ rarg) mfix) ∘ dbody) mfix ->
     Ee.cunfold_fix mfix idx = Some (n, f) ->
-    isEtaExp f.
+    isEtaExp [] f.
   Proof.
-    intros heta.
+    intros hcl heta.
     unfold Ee.cunfold_fix.
     destruct nth_error eqn:heq => //.
     intros [= <- <-] => /=.
-    apply isEtaExp_substl.
-    now apply isEtaExp_fix_subst.
-    eapply forallb_nth_error in heta; tea.
-    now erewrite heq in heta.
+    eapply isEtaExp_fixsubstl.
+    - cbn. solve_all. unfold EAst.test_def. eapply closed_upwards; eauto. lia.
+    - solve_all.
+    - solve_all. eapply All_nth_error in heta as []; eauto.
+      now rewrite app_nil_r.
+      Unshelve. eauto.
   Qed.
   
   Lemma isEtaExp_cunfold_cofix mfix idx n f : 
-    forallb (isEtaExp ∘ dbody) mfix ->
+    forallb (closedn 0 ∘ dbody) mfix ->
+    forallb (isEtaExp (repeat 0 #|mfix|) ∘ dbody) mfix ->
     Ee.cunfold_cofix mfix idx = Some (n, f) ->
-    isEtaExp f.
+    isEtaExp [] f.
   Proof.
-    intros heta.
+    intros hcl heta.
     unfold Ee.cunfold_cofix.
     destruct nth_error eqn:heq => //.
     intros [= <- <-] => /=.
-    apply isEtaExp_substl.
-    now apply isEtaExp_cofix_subst.
-    eapply forallb_nth_error in heta; tea.
-    now erewrite heq in heta.
+    eapply isEtaExp_substl.
+    4:{ solve_all. eapply nth_error_all in heta; eauto. rewrite app_nil_r. eapply heta. }
+    - len. now rewrite cofix_subst_length.
+    - unfold cofix_subst. generalize #|mfix|. clear - hcl. induction n; econstructor; eauto.
+      cbn. solve_all. eapply closed_upwards; eauto. lia.
+    - eapply isEtaExp_cofix_subst in heta. solve_all.
+  Qed.
+
+  Lemma isEtaExp_tApp Γ f u : isEtaExp Γ (mkApps f u) -> 
+    let (hd, v) := decompose_app (mkApps f u) in
+    match expanded_head_viewc hd with
+      | expanded_head_construct ind i => isEtaExp_app ind i #|v| && forallb (isEtaExp Γ) v
+      | expanded_head_fix mfix idx => isEtaExp_fixapp mfix idx #|v| && forallb (fun x => isEtaExp (rev_map (S ∘ rarg) mfix ++ Γ) x.(dbody)) mfix && forallb (isEtaExp Γ) v
+      | expanded_head_rel n => (nth n Γ 0 <=? List.length v) && forallb (fun x => isEtaExp Γ x) v
+      | expanded_head_other t discr => isEtaExp Γ hd && forallb (isEtaExp Γ) v
+      end. (* 
+    | expanded_head_construct kn c => isEtaExp_app Σ kn c #|args| && forallb (isEtaExp Σ) args
+    | expanded_head_fix mfix idx => isEtaExp_fixapp mfix idx #|args| && forallb mfix (fun x => isEtaExp Σ x.(dbody)) && forallb (isEtaExp Σ) args
+    | expanded_head_rel n => (nth n Γ 0 <=? List.length v) && forallb (fun x => isEtaExp Γ x) v
+    | expanded_head_other u discr => isEtaExp Σ hd && forallb (isEtaExp Σ) args
+    end. *)
+  Proof.
+    destruct decompose_app eqn:da.
+    rewrite (decompose_app_inv da).
+    pose proof (decompose_app_notApp _ _ _ da).
+    intros eq.
+    rewrite isEtaExp_mkApps in eq; eauto.
   Qed.
 
 End isEtaExp.
@@ -411,376 +819,6 @@ Module GlobalContextMap.
 End GlobalContextMap.
 Coercion GlobalContextMap.global_decls : GlobalContextMap.t >-> global_declarations.
 
-(* 
-Section AllInP.
-  Context {A : Type}.
-
-  Equations forallb_InP (l : list A) (H : forall x : A, In x l -> bool) : bool :=
-  | nil, _ := true ;
-  | (cons x xs), H := (H x _) && (forallb_InP xs (fun x inx => H x _)).
-End AllInP.
-
-Lemma forallb_InP_spec {A} (f : A -> bool) (l : list A) :
-  forallb_InP l (fun x _ => f x) = List.forallb f l.
-Proof.
-  remember (fun x _ => f x) as g.
-  funelim (forallb_InP l g) => //; simpl. f_equal.
-  now rewrite (H0 f).
-Qed.
-
-Section MapInP.
-  Context {A B : Type}.
-
-  Equations map_InP (l : list A) (f : forall x : A, In x l -> B) : list B :=
-  map_InP nil _ := nil;
-  map_InP (cons x xs) f := cons (f x _) (map_InP xs (fun x inx => f x _)).
-End MapInP.
-
-Lemma map_InP_spec {A B : Type} (f : A -> B) (l : list A) :
-  map_InP l (fun (x : A) _ => f x) = List.map f l.
-Proof.
-  remember (fun (x : A) _ => f x) as g.
-  funelim (map_InP l g) => //; simpl. f_equal. cbn in H.
-  now rewrite (H f0).
-Qed.
-
-Lemma In_size {A B} {x : A} {l : list A} (proj : A -> B) (size : B -> nat) : 
-  In x l -> size (proj x) < S (list_size (size ∘ proj) l).
-Proof.
-  induction l; cbn => //.
-  intros [->|hin]. lia. specialize (IHl hin); lia.
-Qed.
-
-Equations discr_construct (t : term) : Prop :=
-discr_construct (tConstruct ind n) := False ;
-discr_construct _ := True.
-
-Inductive construct_view : term -> Type :=
-| view_construct : forall ind n, construct_view (tConstruct ind n)
-| view_other : forall t, discr_construct t -> construct_view t.
-
-Equations construct_viewc t : construct_view t :=
-construct_viewc (tConstruct ind n) := view_construct ind n ;
-construct_viewc t := view_other t I.
-
-Section isEtaExp.
-  Context (Σ : global_context).
-  Definition lookup_minductive kn : option mutual_inductive_body :=
-    decl <- ETyping.lookup_env Σ kn;; 
-    match decl with
-    | ConstantDecl _ => None
-    | InductiveDecl mdecl => ret mdecl
-    end.
-
-  Definition lookup_inductive kn : option (mutual_inductive_body * one_inductive_body) :=
-    mdecl <- lookup_minductive (inductive_mind kn) ;;
-    idecl <- nth_error mdecl.(ind_bodies) (inductive_ind kn) ;;
-    ret (mdecl, idecl).
-  
-  Definition lookup_inductive_pars kn : option nat := 
-    mdecl <- lookup_minductive kn ;;
-    ret mdecl.(ind_npars).
-  
-  Definition lookup_constructor_pars_args kn c : option (nat * nat) := 
-    '(mdecl, idecl) <- lookup_inductive kn ;;
-    cdecl <- nth_error idecl.(ind_ctors) c ;;
-    ret (mdecl.(ind_npars), cdecl.2).
-    
-  Definition isEtaExp_app ind c k :=
-    match lookup_constructor_pars_args ind c with
-    | Some (npars, nargs) => leb (npars + nargs) k
-    | None => false
-    end.
-    
-  Import TermSpineView.
-
-  Equations? isEtaExp (e : EAst.term) : bool
-    by wf e (fun x y : EAst.term => size x < size y) :=
-  | e with TermSpineView.view e := {
-    | tRel i => true
-    | tEvar ev args => forallb_InP args (fun x H => isEtaExp x)
-    | tLambda na M => isEtaExp M
-    | tApp u v napp nnil with construct_viewc u := 
-      { | view_construct ind i => isEtaExp_app ind i (List.length v) && forallb_InP v (fun x H => isEtaExp x)
-        | view_other _ _ => isEtaExp u && forallb_InP v (fun x H => isEtaExp x) }
-    | tLetIn na b b' => isEtaExp b && isEtaExp b'
-    | tCase ind c brs => isEtaExp c && forallb_InP brs (fun x H => isEtaExp x.2)
-    | tProj p c => isEtaExp c
-    | tFix mfix idx => forallb_InP mfix (fun x H => isEtaExp x.(dbody))
-    | tCoFix mfix idx => forallb_InP mfix (fun x H => isEtaExp x.(dbody))
-    | tBox => true
-    | tVar _ => true
-    | tConst _ => true
-    | tConstruct ind i => isEtaExp_app ind i 0 }.
-  Proof.
-    all:try lia.
-    all:try apply (In_size); tea.
-    all:try lia.
-    - now apply (In_size id size). 
-    - rewrite size_mkApps.
-      change (fun x => size (id x)) with size in H. cbn.
-      now apply (In_size id size).
-    - now eapply size_mkApps_f.
-    - change (fun x => size (id x)) with size in H.
-      eapply (In_size id size) in H. unfold id in H.
-      change (fun x => size x) with size in H. 
-      pose proof (size_mkApps_l napp nnil). lia.
-    - eapply (In_size snd size) in H. cbn in H; lia.
-  Qed.
-  
-  Lemma isEtaExp_app_mon ind c i i' : i <= i' -> isEtaExp_app ind c i -> isEtaExp_app ind c i'.
-  Proof.
-    intros le.
-    unfold isEtaExp_app.
-    destruct lookup_constructor_pars_args as [[pars args]|]=> //.
-    do 2 elim: Nat.leb_spec => //. lia.
-  Qed.
-
-End isEtaExp.
-Global Hint Rewrite @forallb_InP_spec : isEtaExp.
-
-Opaque isEtaExp.
-
-Lemma In_All {A} {P : A -> Type} l : 
-(∀ x : A, In x l -> P x) -> All P l.
-Proof.
-induction l; cbn; constructor; auto.
-Qed.
-
-Ltac toAll := 
-repeat match goal with 
-  | [ H : forall x, In x ?l -> _ |- _ ] => eapply In_All in H
-end.
-
-Section something.
-
-Context (Σ : global_context).
-
-Hint Rewrite @forallb_InP_spec : isEtaExp.
-Transparent isEtaExp_unfold_clause_1.
-
-Lemma isEtaExp_mkApps_nonnil f v :
-  ~~ isApp f -> v <> [] ->
-  isEtaExp Σ (mkApps f v) = match construct_viewc f with 
-    | view_construct ind i => isEtaExp_app Σ ind i #|v| && forallb (isEtaExp Σ) v
-    | view_other t discr => isEtaExp Σ f && forallb (isEtaExp Σ) v
-  end.
-Proof.
-  rewrite isEtaExp_equation_1.
-  intros napp hv.
-  destruct (TermSpineView.view_mkApps (TermSpineView.view (mkApps f v)) napp hv) as [hna [hv' ->]].
-  cbn. destruct (construct_viewc f); cbn; simp isEtaExp => //.
-Qed.
-
-Lemma isEtaExp_mkApps f v : ~~ isApp f ->
-  isEtaExp Σ (mkApps f v) = match construct_viewc f with 
-    | view_construct ind i => isEtaExp_app Σ ind i #|v| && forallb (isEtaExp Σ) v
-    | view_other t discr => isEtaExp Σ f && forallb (isEtaExp Σ) v
-  end.
-Proof.
-  intros napp.
-  destruct v using rev_case; cbn.
-  - destruct construct_viewc; rewrite andb_true_r //.
-  - rewrite isEtaExp_mkApps_nonnil //. now destruct v; cbn; congruence.
-Qed.
-
-Lemma isEtaExp_Constructor ind i v :
-  isEtaExp Σ (mkApps (tConstruct ind i) v) = isEtaExp_app Σ ind i #|v| && forallb (isEtaExp Σ) v.
-Proof.
-  rewrite isEtaExp_mkApps //.
-Qed.
-
-Lemma isEtaExp_mkApps_intro t l : isEtaExp Σ t -> All (isEtaExp Σ) l -> isEtaExp Σ (mkApps t l).
-Proof.
-  revert t; induction l using rev_ind; auto.
-  intros t et a; eapply All_app in a as [].
-  depelim a0. clear a0.
-  destruct (decompose_app t) eqn:da.
-  rewrite (decompose_app_inv da) in et *.
-  pose proof (decompose_app_notApp _ _ _ da).
-  destruct l0. cbn.
-  - rewrite isEtaExp_mkApps //.
-    destruct construct_viewc. cbn. len.
-    rtoProp; repeat solve_all. cbn in et. simp isEtaExp in et.
-    eapply isEtaExp_app_mon; tea; lia.
-    eapply All_app_inv; eauto. rewrite et forallb_app /=.
-    rtoProp; repeat solve_all.
-  - rewrite isEtaExp_mkApps in et => //.
-    destruct construct_viewc.
-    rewrite -mkApps_app. rewrite isEtaExp_Constructor.
-    cbn. cbn. rtoProp; solve_all.
-    eapply isEtaExp_app_mon; tea. cbn. len. lia. now depelim H1.
-    depelim H1. solve_all. eapply All_app_inv => //.
-    eapply All_app_inv => //. eauto.
-    rewrite -mkApps_app. rewrite isEtaExp_mkApps //.
-    destruct (construct_viewc t0) => //.
-    move/andP: et => [] -> /=. rtoProp; solve_all.
-    rewrite forallb_app. rtoProp; repeat solve_all.
-    eapply All_app_inv; eauto.
-Qed.
-
-Lemma csubst_mkApps {a k f l} : csubst a k (mkApps f l) = mkApps (csubst a k f) (map (csubst a k) l).
-Proof.
-  induction l using rev_ind; simpl; auto.
-  rewrite mkApps_app /= IHl.
-  now rewrite -[EAst.tApp _ _](mkApps_app _ _ [_]) map_app.
-Qed.
-
-Lemma etaExp_csubst a k b : 
-  isEtaExp Σ a -> isEtaExp Σ b -> isEtaExp Σ (ECSubst.csubst a k b).
-Proof.
-  funelim (isEtaExp Σ b); cbn; simp isEtaExp; rewrite -?isEtaExp_equation_1; eauto;
-    toAll; repeat solve_all.
-  - intros. destruct Nat.compare => //.
-  - move/andP: H2 => [] etab etab'.
-    apply/andP. split; eauto.
-  - rtoProp. intuition eauto.
-    solve_all.
-  - move/andP: H1 => [] etaexp h.
-    rewrite csubst_mkApps /=.
-    rewrite isEtaExp_Constructor. solve_all.
-    rewrite map_length. rtoProp; solve_all. solve_all.
-  - rewrite csubst_mkApps /=.
-    move/andP: H2 => [] eu ev.
-    specialize (H _ k H1 eu).
-    eapply isEtaExp_mkApps_intro => //. solve_all.
-Qed.
-
-End something.
-
-Definition isEtaExp_constant_decl Σ cb := 
-  option_default (isEtaExp Σ) cb.(cst_body) true.
-
-Definition isEtaExp_decl Σ d :=
-  match d with
-  | ConstantDecl cb => isEtaExp_constant_decl Σ cb
-  | InductiveDecl idecl => true
-  end.
-
-Fixpoint isEtaExp_env (Σ : EAst.global_declarations) := 
-  match Σ with 
-  | [] => true
-  | decl :: Σ => isEtaExp_decl Σ decl.2 && isEtaExp_env Σ
-  end.
-
-(* Lemma strip_extends Σ Σ' : extends Σ Σ' ->
-  strip Σ t = strip Σ' t. *)
-
-Lemma isEtaExp_tApp Σ f u : isEtaExp Σ (mkApps f u) -> 
-  let (hd, args) := decompose_app (mkApps f u) in
-  match construct_viewc hd with
-  | view_construct kn c => isEtaExp_app Σ kn c #|args| && forallb (isEtaExp Σ) args
-  | view_other u discr => isEtaExp Σ hd && forallb (isEtaExp Σ) args
-  end.
-Proof.
-  destruct decompose_app eqn:da.
-  rewrite (decompose_app_inv da).
-  pose proof (decompose_app_notApp _ _ _ da).
-  destruct l. cbn -[isEtaExp].
-  intros eq; rewrite eq.
-  destruct (construct_viewc t) => //. simp isEtaExp in eq; now rewrite eq.
-  assert (t0 :: l <> []) by congruence.
-  revert da H0. generalize (t0 :: l). clear t0 l; intros l.
-  intros da nnil.
-  rewrite isEtaExp_mkApps //.
-Qed. *)
-
-From MetaCoq.Template Require Import config utils BasicAst Universes.
-From MetaCoq.Erasure Require Import EAst ETyping EAstUtils.
-
-Section expanded.
-
-Variable Σ : global_declarations.
-
-Local Unset Elimination Schemes.
-
-Inductive expanded : term -> Prop :=
-| expanded_tRel (n : nat) : expanded (tRel n)
-| expanded_tVar (id : ident) : expanded (tVar id)
-| expanded_tEvar (ev : nat) (args : list term) : Forall expanded args -> expanded (tEvar ev args)
-| expanded_tLambda (na : name) (body : term) : expanded body -> expanded (tLambda na body)
-| expanded_tLetIn (na : name) (def : term)(body : term) : expanded def -> expanded body -> expanded (tLetIn na def body)
-| expanded_mkApps (f : term) (args : list term) : ~ isConstruct f -> expanded f -> Forall expanded args -> expanded (mkApps f args)
-| expanded_tConst (c : kername) : expanded (tConst c)
-| expanded_tCase (ind : inductive) (pars : nat) (discr : term) (branches : list (list name × term)) : 
-    expanded discr -> Forall (fun br => expanded br.2) branches -> expanded (tCase (ind, pars) discr branches)
-| expanded_tProj (proj : projection) (t : term) : expanded t -> expanded (tProj proj t)
-| expanded_tFix (mfix : mfixpoint term) (idx : nat) args d : 
-  Forall (fun d => expanded d.(dbody)) mfix ->
-  Forall expanded args ->
-  args <> [] ->
-  nth_error mfix idx = Some d ->
-  #|args| > d.(rarg) ->
-  expanded (mkApps (tFix mfix idx) args)
-| expanded_tCoFix (mfix : mfixpoint term) (idx : nat) : Forall (fun d => expanded d.(dbody)) mfix -> expanded (tCoFix mfix idx)
-| expanded_tConstruct_app ind idx mind idecl cname c args :
-    declared_constructor Σ (ind, idx) mind idecl (cname, c) ->
-    #|args| >= ind_npars mind + c -> 
-    Forall expanded args ->
-    expanded (mkApps (tConstruct ind idx) args)
-| expanded_tBox : expanded tBox.
-
-End expanded.
-
-Lemma expanded_ind :
-forall (Σ : global_declarations) (P : term -> Prop),
-(forall n : nat, P (tRel n)) ->
-(forall id : ident, P (tVar id)) ->
-(forall (ev : nat) (args : list term), Forall (expanded Σ) args -> Forall P args -> P (tEvar ev args)) ->
-(forall (na : name) (body : term),
- expanded Σ body -> P body -> P (tLambda na body)) ->
-(forall (na : name) (def body : term),
- expanded Σ def ->
- P def -> expanded Σ body -> P body -> P (tLetIn na def body)) ->
-(forall (f4 : term) (args : list term),
- ~ isConstruct f4 ->
- expanded Σ f4 -> P f4 -> Forall (expanded Σ) args -> Forall P args -> P (mkApps f4 args)) ->
-(forall c : kername, P (tConst c)) ->
-(forall (ind : inductive) (pars : nat) (discr : term)
-   (branches : list (list name × term)),
- expanded Σ discr ->
- P discr ->
- Forall (fun br : list name × term => expanded Σ br.2) branches ->
- Forall (fun br : list name × term => P br.2) branches ->
- P (tCase (ind, pars) discr branches)) ->
-(forall (proj : projection) (t : term),
- expanded Σ t -> P t -> P (tProj proj t)) ->
-(forall (mfix : mfixpoint term) (idx : nat) d args, 
- Forall (fun d => expanded Σ d.(dbody)) mfix -> 
- Forall (fun d => P d.(dbody)) mfix -> 
- Forall (expanded Σ) args ->
- Forall P args ->
- args <> [] ->
- nth_error mfix idx = Some d ->
- #|args| > d.(rarg) ->
- expanded Σ (mkApps (tFix mfix idx) args) ->
- P (mkApps (tFix mfix idx) args)) ->
-(forall (mfix : mfixpoint term) (idx : nat),
- Forall (fun d : def term => expanded Σ (dbody d)) mfix ->  Forall (fun d : def term => P (dbody d)) mfix ->
- P (tCoFix mfix idx)) ->
-(forall (ind : inductive) (idx : nat) (mind : mutual_inductive_body)
-   (idecl : one_inductive_body) (cname : ident) (c : nat) 
-   (args : list term),
- declared_constructor Σ (ind, idx) mind idecl (cname, c) ->
- #|args| >= ind_npars mind + c -> Forall (expanded Σ) args -> Forall P args -> P (mkApps (tConstruct ind idx) args)) ->
-(P tBox) ->
-forall t : term, expanded Σ t -> P t.
-Proof. 
-  intros. revert t H12.
-  fix f 2.
-  intros t Hexp. destruct Hexp; eauto.
-  - eapply H1; eauto. induction H12; econstructor; cbn in *; eauto.
-  - eapply H4; eauto. induction H13; econstructor; cbn in *; eauto.
-  - eapply H6; eauto. induction H12; econstructor; cbn in *; eauto.
-  - eapply H8; eauto.
-    + clear - H12 f. induction H12; econstructor; cbn in *; eauto.
-    + clear - H13 f. induction H13; econstructor; cbn in *; eauto.
-    + eapply expanded_tFix; eauto.
-  - eapply H9; eauto. induction H12; econstructor; cbn in *; eauto.
-  - eapply H10; eauto. clear - H14 f. induction H14; econstructor; cbn in *; eauto.
-Qed.
-
-Local Hint Constructors expanded : core .
 Tactic Notation "simp_eta" "in" hyp(H) := simp isEtaExp in H; rewrite -?isEtaExp_equation_1 in H.
 Ltac simp_eta := simp isEtaExp; rewrite -?isEtaExp_equation_1.
 
@@ -809,12 +847,14 @@ Proof.
   intros. eapply isEtaExp_app_expanded. eauto 8.
 Qed.
 
-Lemma isEtaExp_expanded Σ t :
-  isEtaExp Σ t -> expanded Σ t.
+Lemma isEtaExp_expanded Σ Γ t :
+  isEtaExp Σ Γ t -> expanded Σ Γ t.
 Proof.
-  funelim (isEtaExp Σ t); intros; solve_all; eauto.
+  funelim (isEtaExp Σ Γ t); intros; solve_all; eauto.
+  - econstructor. now eapply Nat.eqb_eq.
+  - todo "tVar".
   - rewrite forallb_InP_spec in H0. eapply forallb_Forall in H0. eapply In_All in H.
-    econstructor. solve_all.
+    todo "tEvar".
   - eapply andb_true_iff in H1 as []; eauto.
   - eapply isEtaExp_app_expanded in H as (? & ? & ? & ? & ? & ?).
     eapply expanded_tConstruct_app with (args := []); eauto.
@@ -831,7 +871,11 @@ Proof.
   - rtoProp. rewrite forallb_InP_spec in H2. rewrite forallb_InP_spec in H3. eapply In_All in H. eapply In_All in H0. 
     unfold isEtaExp_fixapp in H1. destruct nth_error eqn:E; try congruence.
     eapply expanded_tFix.
-    all: try now solve_all. eapply Nat.ltb_lt in H1. lia.
+    all: try now solve_all.
+    eapply Nat.ltb_lt in H1. lia.
+  - rtoProp. econstructor. eapply Nat.leb_le; eauto.  rewrite forallb_InP_spec in H1.
+    eapply Forall_forall. solve_all. eapply H; eauto.
+    eapply All_Forall, Forall_forall in H1; eauto.
   - eapply andb_true_iff in H1 as []. rewrite forallb_InP_spec in H2. eapply forallb_Forall in H2.
     econstructor.
     + destruct u; inv Heq; eauto.
@@ -839,20 +883,453 @@ Proof.
     + eapply In_All in H0. solve_all.
 Qed.
 
-Lemma expanded_isEtaExp Σ t :
-  expanded Σ t -> isEtaExp Σ t.
+Lemma expanded_isEtaExp Σ Γ t :
+  expanded Σ Γ t -> isEtaExp Σ Γ t.
 Proof.
   induction 1; simp_eta; eauto.
   all: try now (
     (try (eapply andb_true_iff; split; eauto));
     (try eapply forallb_Forall); 
     eauto).
-  - eapply isEtaExp_mkApps_intro; eauto. solve_all.
-  - rewrite isEtaExp_mkApps //. cbn [cc_viewc]. rtoProp. repeat split.
+  - eapply Nat.eqb_eq; eauto.
+  - rewrite isEtaExp_mkApps //. cbn [expanded_head_viewc].
+    rtoProp. split. 2: solve_all. now eapply Nat.leb_le.
+  - eapply isEtaExp_mkApps_intro; eauto. solve_all. 
+  - rewrite isEtaExp_mkApps //. cbn [expanded_head_viewc]. rtoProp. repeat split.
     + unfold isEtaExp_fixapp. rewrite H4. eapply Nat.ltb_lt. lia.
-    + rewrite forallb_InP_spec. solve_all.
+    + solve_all.
     + solve_all.
   - rewrite isEtaExp_Constructor. eapply andb_true_iff.
     split. 2: eapply forallb_Forall.
     2: solve_all. eapply expanded_isEtaExp_app_; eauto.
 Qed.
+
+Definition isEtaExp_constant_decl Σ cb := 
+  option_default (isEtaExp Σ []) cb.(cst_body) true.
+
+Definition isEtaExp_decl Σ d :=
+  match d with
+  | ConstantDecl cb => isEtaExp_constant_decl Σ cb
+  | InductiveDecl idecl => true
+  end.
+
+Fixpoint isEtaExp_env (Σ : global_declarations) := 
+  match Σ with 
+  | [] => true
+  | decl :: Σ => isEtaExp_decl Σ decl.2 && isEtaExp_env Σ
+  end.
+
+
+Lemma closedn_mkApps k f l : closedn k (mkApps f l) = closedn k f && forallb (closedn k) l.
+Proof.
+  induction l in f |- *; cbn; auto.
+  - now rewrite andb_true_r.
+  - now rewrite IHl /= andb_assoc.
+Qed.
+
+Lemma lookup_inductive_pars_constructor_pars_args Σ {ind n pars args} : 
+  lookup_constructor_pars_args Σ ind n = Some (pars, args) ->
+  lookup_inductive_pars Σ (inductive_mind ind) = Some pars.
+Proof.
+  rewrite /lookup_constructor_pars_args /lookup_inductive_pars.
+  rewrite /lookup_inductive. destruct lookup_minductive => //.
+  cbn. do 2 destruct nth_error => //. congruence.
+Qed.
+
+Lemma eval_construct  {fl : Ee.WcbvFlags} Σ kn c args e : 
+  Ee.eval Σ (mkApps (tConstruct kn c) args) e -> ∑ args', (e = mkApps (tConstruct kn c) args') × All2 (Ee.eval Σ) args args'.
+Proof.
+  revert e; induction args using rev_ind; intros e.
+  - intros ev. depelim ev. exists []=> //.
+  - intros ev. rewrite mkApps_app /= in ev.
+    depelim ev; try solve_discr.
+    destruct (IHargs _ ev1) as [? []]. solve_discr.
+    all:try specialize (IHargs _ ev1) as [? []]; try solve_discr.
+    * subst f'. 
+      exists (x0 ++ [a'])%list.
+      rewrite mkApps_app /= //.
+      cbn in i. split => //. eapply All2_app; eauto.
+    * now cbn in i.
+Qed.
+
+Lemma app_tip_nil {A} (l : list A) (x : A) : (l ++ [x])%list <> [].
+Proof.
+  destruct l; cbn; congruence.
+Qed.
+
+Lemma eval_mkApps_Construct {fl : Ee.WcbvFlags} Σ kn c args args' : 
+  All2 (Ee.eval Σ) args args' ->
+  Ee.eval Σ (mkApps (tConstruct kn c) args) (mkApps (tConstruct kn c) args').
+Proof.
+  revert args'. induction args using rev_ind; intros args'; destruct args' using rev_case; intros a.
+  - depelim a. constructor => //.
+  - depelim a. cbn. now apply app_tip_nil in H.
+  - depelim a. now apply app_tip_nil in H.
+  - eapply All2_app_inv in a as []. 2:{ eapply All2_length in a. len in a. cbn in a. lia. } 
+    depelim a0. clear a0. rewrite !mkApps_app /=.
+    constructor; auto.
+    destruct args' using rev_ind; try now rewrite ?mkApps_app; cbn; destruct Ee.with_guarded_fix; eauto.
+    cbn. rewrite Ee.isFixApp_mkApps; eauto.
+    cbn. try now rewrite ?mkApps_app; cbn; destruct Ee.with_guarded_fix; eauto.
+Qed.
+
+Definition remove_last {A} (args : list A) := 
+  List.firstn (#|args| - 1) args.
+
+Lemma remove_last_app {A} (l : list A) x : 
+  remove_last (l ++ [x]) = l.
+Proof.
+  unfold remove_last. cbn. len.
+  replace (#|l| + 1 -1) with #|l| by lia.
+  rewrite firstn_app Nat.sub_diag /= firstn_all app_nil_r //.
+Qed.
+
+Arguments isEtaExp : simpl never.
+
+Lemma isEtaExp_tApp' {Σ} {Γ} {f u} : isEtaExp Σ Γ (tApp f u) -> 
+  let (hd, args) := decompose_app (tApp f u) in
+  match expanded_head_viewc hd with
+  | expanded_head_construct kn c =>
+    args <> [] /\ f = mkApps hd (remove_last args) /\ u = last args u /\ 
+    isEtaExp_app Σ kn c #|args| && forallb (isEtaExp Σ Γ) args
+  | expanded_head_fix mfix idx => 
+    args <> [] /\ f = mkApps hd (remove_last args) /\ u = last args u /\ 
+    isEtaExp_fixapp mfix idx #|args| && forallb (fun d => isEtaExp Σ (rev_map (fun  d => 1 + d.(rarg)) mfix ++ Γ) d.(dbody)) mfix && forallb (isEtaExp Σ Γ) args
+  | expanded_head_rel n => 
+    args <> [] /\ f = mkApps hd (remove_last args) /\ u = last args u /\ 
+    (nth n Γ 0 <=? List.length args) && forallb (fun x => isEtaExp Σ Γ x) args
+  | expanded_head_other _ discr => 
+    [&& isEtaExp Σ Γ hd, forallb (isEtaExp Σ Γ) args, isEtaExp Σ Γ f & isEtaExp Σ Γ u]
+  end.
+Proof.
+  move/(isEtaExp_tApp Σ Γ f [u]).
+  cbn -[decompose_app]. destruct decompose_app eqn:da.
+  destruct expanded_head_viewc eqn:cv => //.
+  - intros ->.
+    pose proof (decompose_app_inv da).
+    pose proof (decompose_app_notApp _ _ _ da).
+    destruct l using rev_case. cbn. intuition auto. solve_discr. noconf H.
+    rewrite mkApps_app in H. noconf H.
+    rewrite remove_last_app last_last. intuition auto.
+    destruct l; cbn in *; congruence.
+  - intros Hfix.
+    pose proof (decompose_app_inv da).
+    pose proof (decompose_app_notApp _ _ _ da).
+    destruct l using rev_case. cbn. intuition auto. solve_discr. noconf H. noconf H.
+    rewrite mkApps_app in H. noconf H.
+    rewrite remove_last_app last_last. intuition auto.
+    destruct l; cbn in *; congruence.
+  - intros ->.
+    pose proof (decompose_app_inv da).
+    pose proof (decompose_app_notApp _ _ _ da).
+    destruct l using rev_case. cbn. intuition auto. solve_discr. noconf H.
+    rewrite mkApps_app in H. noconf H.
+    rewrite remove_last_app last_last. intuition auto.
+    destruct l; cbn in *; congruence.
+  - pose proof (decompose_app_inv da).
+    pose proof (decompose_app_notApp _ _ _ da).
+    destruct l using rev_case. cbn. intuition auto. destruct t => //.
+    rewrite mkApps_app in H. noconf H.
+    move=> /andP[] etat. rewrite forallb_app => /andP[] etal /=.
+    rewrite andb_true_r => etaa. rewrite etaa andb_true_r.
+    rewrite etat etal. cbn. rewrite andb_true_r.
+    eapply isEtaExp_mkApps_intro; auto; solve_all.
+Qed.
+
+Lemma decompose_app_tApp_split f a hd args :
+  decompose_app (tApp f a) = (hd, args) -> f = mkApps hd (remove_last args) /\ a = last args a.
+Proof.
+  unfold decompose_app. cbn.
+  move/decompose_app_rec_inv' => [n [napp [hskip heq]]].
+  rewrite -(firstn_skipn n args).
+  rewrite -hskip. rewrite last_last; split => //.
+  rewrite heq. f_equal.
+  now rewrite remove_last_app.
+Qed.
+
+Lemma remove_last_last {A} (l : list A) (a : A) : l <> [] ->
+  l = (remove_last l ++ [last l a])%list.
+Proof.
+  induction l using rev_ind.
+  congruence.
+  intros. rewrite remove_last_app last_last //.
+Qed.
+
+Lemma forallb_repeat {A} {p : A -> bool} {a : A} {n} : 
+  p a ->
+  forallb p (repeat a n).
+Proof.
+  intros pa.
+  induction n; cbn; auto.
+  now rewrite pa IHn.
+Qed.
+
+Lemma isEtaExp_lookup_ext {Σ} {kn d}: 
+  isEtaExp_env Σ ->
+  lookup_env Σ kn = Some d ->
+  ∑ Σ', extends Σ' Σ × isEtaExp_decl Σ' d.
+Proof.
+  induction Σ; cbn.
+  - move=> _; rewrite /declared_constant /lookup_env /= //.
+  - move=> /andP[] etaa etaΣ.
+    destruct a as [kn' d']; cbn in *.
+    rewrite /declared_constant /=; rewrite /eq_kername; destruct kername_eq_dec.
+    * subst kn'. move=> [=]. intros ->.
+      exists Σ. split => //. now exists [(kn, d)].
+    * move=> Hl. destruct (IHΣ etaΣ Hl) as [Σ' [ext eta]].
+      exists Σ'; split => //.
+      destruct ext as [Σ'' ->].
+      now exists ((kn', d')::Σ'').
+Qed.
+
+Lemma isEtaExp_app_extends Σ Σ' ind k n :
+  extends Σ Σ' ->
+  wf_glob Σ' -> 
+  isEtaExp_app Σ ind k n ->
+  isEtaExp_app Σ' ind k n.
+Proof.
+  rewrite /isEtaExp_app.
+  rewrite /lookup_constructor_pars_args /lookup_inductive /lookup_minductive.
+  move=> ext wf.
+  destruct (lookup_env Σ _) eqn:hl => //.
+  rewrite (extends_lookup wf ext hl) /= //.
+Qed.
+
+Lemma isEtaExp_extends Σ Σ' Γ t : 
+  extends Σ Σ' ->
+  wf_glob Σ' ->
+  isEtaExp Σ Γ t ->
+  isEtaExp Σ' Γ t.
+Proof.
+  intros ext wf.
+  funelim (isEtaExp Σ Γ t); simp_eta => //; rtoProp; intuition eauto; rtoProp; intuition auto.
+  - eapply In_All in H; solve_all.
+  - eapply isEtaExp_app_extends; tea.
+  - eapply In_All in H0. solve_all.
+  - eapply In_All in H; solve_all.
+  - eapply In_All in H; solve_all.
+    rewrite isEtaExp_Constructor //. rtoProp; intuition auto.
+    eapply isEtaExp_app_extends; tea.
+    solve_all.
+  - eapply In_All in H, H0. rewrite isEtaExp_mkApps => //.
+    cbn [expanded_head_viewc]. rtoProp. repeat split; eauto.
+    all: solve_all.
+  - eapply In_All in H. rewrite isEtaExp_mkApps => //.
+    cbn [expanded_head_viewc]. rtoProp. repeat split; eauto.
+    all: solve_all.
+  - eapply In_All in H0. apply isEtaExp_mkApps_intro; eauto. solve_all.
+Qed.
+
+Lemma isEtaExp_extends_decl Σ Σ' t : 
+  extends Σ Σ' ->
+  wf_glob Σ' ->
+  isEtaExp_decl Σ t ->
+  isEtaExp_decl Σ' t.
+Proof.
+  intros ext wf; destruct t; cbn => //.
+  rewrite /isEtaExp_constant_decl; destruct (cst_body c) => /= //.
+  now eapply isEtaExp_extends.
+Qed.
+
+Lemma isEtaExp_lookup {Σ kn d}: 
+  isEtaExp_env Σ -> wf_glob Σ ->
+  lookup_env Σ kn = Some d ->
+  isEtaExp_decl Σ d.
+Proof.
+  move=> etaΣ wfΣ.
+  move/(isEtaExp_lookup_ext etaΣ) => [Σ' []] ext hd.
+  now eapply isEtaExp_extends_decl.
+Qed.
+
+Arguments lookup_inductive_pars_constructor_pars_args {Σ ind n pars args}.
+
+Lemma eval_etaexp {fl : Ee.WcbvFlags} {Σ a a'} : 
+  isEtaExp_env Σ ->
+  wf_glob Σ ->
+  closed_env Σ ->
+  closedn 0 a ->
+  Ee.eval Σ a a' -> isEtaExp Σ [] a -> isEtaExp Σ [] a'.
+Proof.
+  intros etaΣ wfΣ HΣcl Hcl.
+  induction 1 using eval_mkApps_rect.
+  all:try simp isEtaExp; rewrite -!isEtaExp_equation_1 => //.
+  - move/isEtaExp_tApp'.
+    destruct decompose_app eqn:da.
+    destruct expanded_head_viewc eqn:vc.
+    * move => [hl [hf [ha /andP[] ise etal]]].
+      rewrite hf in H. eapply eval_construct in H as [? []]. exfalso. solve_discr.
+    * move => [hl [hf [ha /andP[] /andP[] etal etab]]] isel.
+      unfold isEtaExp_fixapp in etal. destruct nth_error eqn:Efix; try easy.
+      (* maybe the new relation does not preserve eta-expandedness? it's certainly hard to prove.
+
+         From H we can get that remove_last l was long enough to trigger evaluation, so the shorter application is still expanded
+      
+      *)
+      rewrite hf in H. eapply IHeval3. admit.
+      eapply etaExp_csubst; eauto. admit.
+      eapply IHeval2. admit.
+      solve_all. admit.
+      simp_eta in IHeval1.
+      eapply IHeval1.
+      subst. cbn in Hcl. rtoProp. eauto.
+      subst. econstructor.
+    * todo "rel".
+    * move/and4P => [] etat etal etaf etaa.
+      move / andP : Hcl => [] Hcl1 Hcl2; fold closedn in *.
+      eapply IHeval3; eauto.
+      { eapply closed_csubst. eapply eval_closed; eauto. eapply eval_closed in H; eauto. }
+      move: (IHeval1 Hcl1 etaf); simp_eta => etab.      
+      eapply etaExp_csubst; eauto.
+      { eapply eval_closed; eauto. }
+  - admit.
+  - move : Hcl => /andP [] Hcl1 Hcl2; fold closedn in *.  
+    rtoProp; intuition eauto.
+    eapply IHeval2. rewrite /iota_red.
+    { eapply closed_substl.
+       eapply eval_closed in H; eauto. rewrite closedn_mkApps in H. rtoProp. solve_all. eapply All_skipn. solve_all.
+      solve_all. eapply All_nth_error in H6 as []; eauto. revert i. len. now rewrite H2.
+    }
+    eapply isEtaExp_substl with (Γ := repeat 0 #|br.1|); eauto.
+    { len. rewrite List.skipn_length repeat_length in H2 |- *. lia. }
+    { eapply eval_closed in H; eauto. rewrite closedn_mkApps in H. rtoProp. solve_all. eapply All_skipn. solve_all. }
+    rewrite isEtaExp_Constructor // in H7. solve_all.
+    eapply All_skipn. move/andP: H7 => []. repeat solve_all.
+    eapply forallb_nth_error in H6; tea.
+    now erewrite H1 in H6.
+  - rtoProp; intuition auto.
+    eapply IHeval2. eapply isEtaExp_substl.
+    now apply forallb_repeat.
+    rewrite H2 in H6. simpl in H6.
+    now move/andP: H6.
+  - intros ise.
+    eapply IHeval3.
+    apply isEtaExp_tApp' in ise.
+    destruct decompose_app eqn:da.
+    destruct (cc_viewc t) eqn:cv.
+    * destruct ise as [? [? []]]. rewrite H4 in H.
+      eapply eval_construct in H as [? []];solve_discr.
+    * todo "fix". 
+    * move/and4P: ise => [] iset isel isef isea.
+      rewrite -[EAst.tApp _ _](mkApps_app _ _ [av]).
+      specialize (IHeval1 isef).
+      rewrite isEtaExp_mkApps // in IHeval1.
+      simp cc_viewc in IHeval1.
+      move: IHeval1 => /andP [] / andP [] evrarg evfix evargs.
+      eapply isEtaExp_mkApps_intro.
+      eapply isEtaExp_cunfold_fix; tea.
+      simp isEtaExp in evfix.
+      eapply All_app_inv. now solve_all. constructor; auto.
+  - intros ise.
+    apply isEtaExp_tApp' in ise.
+    destruct decompose_app eqn:da.
+    destruct (cc_viewc t) eqn:cv.
+    * destruct ise as [? [? []]]. rewrite H4 in H.
+      eapply eval_construct in H as [? []]; solve_discr.
+    * todo "fix".
+    * move/and4P: ise => [] iset isel isef isea.
+      rewrite -[EAst.tApp _ _](mkApps_app _ _ [av]).
+      specialize (IHeval1 isef).
+      rewrite isEtaExp_mkApps // in IHeval1.
+      simp construct_viewc in IHeval1.
+      move: IHeval1 => /andP [] / andP [] evrarg evfix evargs.
+      todo "fix". (* 
+      eapply isEtaExp_mkApps_intro => //.
+      eapply All_app_inv. now solve_all. constructor; auto. *)
+  - move=> /andP[] hdiscr hbrs. specialize (IHeval1 hdiscr).
+    move: IHeval1. rewrite isEtaExp_mkApps // /= => /andP[] hcof hargs.
+    eapply IHeval2. simp_eta. rtoProp; intuition auto.
+    apply isEtaExp_mkApps_intro; solve_all.
+    eapply (isEtaExp_cunfold_cofix _ mfix idx); tea.
+    simp_eta in hcof.
+  -  move=> hdiscr. specialize (IHeval1 hdiscr).
+    move: IHeval1. rewrite isEtaExp_mkApps // /= => /andP[] hcof hargs.
+    eapply IHeval2. simp_eta.
+    apply isEtaExp_mkApps_intro; solve_all.
+    eapply (isEtaExp_cunfold_cofix _ mfix idx); tea.
+    simp_eta in hcof.
+  - move=> _. eapply IHeval. eapply isEtaExp_lookup in H; tea.
+    now move: H; rewrite /isEtaExp_decl /= /isEtaExp_constant_decl H0 /=.
+  - intros hd.
+    eapply IHeval2. specialize (IHeval1 hd).
+    move: IHeval1.
+    rewrite nth_nth_error in H1 *.
+    destruct nth_error eqn:hnth.
+    rewrite isEtaExp_Constructor.
+    destruct args => //. now rewrite nth_error_nil in hnth.
+    move=> /andP[] _ hargs. eapply nth_error_forallb in hnth; tea.
+    depelim H0. now cbn in H1.
+  - move/isEtaExp_tApp'.
+    destruct decompose_app eqn:da.
+    destruct cc_viewc.
+    * move=> [] hl [] hf [] ha /andP[] hl' etal.
+      move: H H0. rewrite hf => H H0.
+      destruct (eval_construct_size H) as [args' []]. subst f'.
+      rewrite -[EAst.tApp _ _](mkApps_app _ _ [a']).
+      rewrite isEtaExp_Constructor.
+      apply/andP; split => //.
+      + len. eapply All2_length in a0. rewrite -a0.
+        rewrite (remove_last_last l a) // in hl'. len in hl'.
+        now cbn in hl'.
+      + solve_all.
+        rewrite (remove_last_last l a) // in etal.
+        eapply All_app in etal as [etal etaa].
+        depelim etaa. clear etaa. rewrite -ha in i.
+        eapply All_app_inv; try constructor; eauto.
+        clear -H0 a0 etal. solve_all.
+        destruct b as [ev Hev]. eapply (H0 _ _ ev) => //. lia.
+    * todo "fix".
+    * move/and4P => [] etat etal etaf etaa.
+      eapply (isEtaExp_mkApps_intro _ f' [a']); eauto.
+Qed.
+
+Lemma isEtaExp_eval Σ {wfl : WcbvFlags} t v  :
+eval Σ t v -> isEtaExp Σ [] t -> isEtaExp Σ [] v.
+Admitted.
+
+Local Hint Resolve isEtaExp_eval : core.
+Local Hint Constructors eval : core.
+
+Arguments eval : clear implicits.
+
+Lemma eval_opt_to_target Σ t v  :
+@eval opt_wcbv_flags Σ t v -> isEtaExp Σ [] t -> @eval target_wcbv_flags Σ t v.
+Proof.
+intros H. depind H; intros Hexp; eauto.
+- todo "box".
+- todo "lambda".
+- simp_eta in Hexp. rtoProp. econstructor. eauto. eapply IHeval2. todo "isEtaExp csubst".
+- todo "case".
+- todo "case".
+- destruct argsv.
+  + cbn -[isEtaExp] in *. todo "impossible due to expansion".
+  + eapply eval_trans. eapply eval_app_cong.
+    * eapply IHeval1. todo "exp".
+    * cbn. destruct argsv using rev_ind; cbn; try eauto. now rewrite mkApps_app. 
+    * eapply IHeval2. todo "exp". 
+    * replace (tApp (mkApps fn (t :: argsv)) av) with (mkApps (tApp fn t) (argsv ++ [av])) in IHeval3 by now rewrite mkApps_app.
+      replace (tApp (mkApps (tFix mfix idx) (t :: argsv)) av) with (mkApps (tApp (tFix mfix idx) t) (argsv ++ [av])) by now rewrite mkApps_app.
+      forward IHeval3. todo "exp".
+      revert IHeval3. generalize (argsv ++ [av])%list. clear - e. intros l.
+      revert res.
+      induction l using rev_ind.
+      -- cbn in *. intros. eapply eval_fix'; eauto.
+      -- rewrite !mkApps_app; cbn. intros res H.
+         eapply eval_trans.
+         eapply eval_mkApps_inv with (args := [x]) in H as (? & ? & ?).
+         eapply eval_app_cong_tApp. eapply IHl; eauto.
+         cbn in *. eauto.
+         eapply value_final, eval_to_value; eauto.
+- todo "impossible due to expansion".
+- cbn in unguarded. congruence.
+- todo "case".
+- todo "proj".
+- todo "const".
+- todo "proj".
+- todo "proj".
+- eapply eval_app_cong.
+  + eapply IHeval1. todo "exp".
+  + eapply IHeval2. todo "exp".
+  + destruct f'; cbn in *; eauto.
+
+Qed.
+ 
